switches to mathlibs Equiv.swap to build coherent picture wrt permutations

Cslib/Languages/LambdaCalculus/Named/Untyped/AlphaEquivDefs.lean
@@ -57,19 +57,8 @@ variable {Var : Type u} [DecidableEq Var] [HasFresh Var]
 
 namespace LambdaCalculus.Named.Untyped.Term
 
-/-- The action of the transposition `(x y)` on a term: simultaneously swaps all occurrences
-of `x` and `y`. Corresponds to `(x y) · E` in [Crole2012] (Section 2).
--/
-def swap (m : Term Var) (x y : Var) : Term Var :=
-  match m with
-  | var z => var (if z = x then y else if z = y then x else z)
-  | abs z m' => abs (if z = x then y else if z = y then x else z) (m'.swap x y)
-  | app n1 n2 => app (n1.swap x y) (n2.swap x y)
 
 /-- The action `π · E` of a permutation on a term, as used in [Crole2012].
-
-`swap` is is one special case of a permutation: the transposition that exchanges exactly two atoms
-a and b and fixes everything else.
 
 Since some lemmas in section 6 are proven for general permutations, we have to introduce
 this notion here aswell and derive the special case using `swap` accordingly.
@@ -79,6 +68,14 @@ def permute (m : Term Var) (π : Equiv.Perm Var) : Term Var :=
   | var x => var (π x)
   | abs x m => abs (π x) (m.permute π)
   | app m n => app (m.permute π) (n.permute π)
+
+/-- The action of the transposition `(x y)` on a term: simultaneously swaps all occurrences
+of `x` and `y`. Corresponds to `(x y) · E` in [Crole2012] (Section 2).
+
+`swap` is is one special case of a permutation: the transposition that exchanges exactly two atoms
+a and b and fixes everything else.
+-/
+def swap (m : Term Var) (x y : Var) : Term Var := m.permute (Equiv.swap x y)
 
 /-- **Definition 3.2** [Crole2012]: `∼p#` - α-equivalence via permutation with freshness
 side condition.
